experiments/003_bytecode_layer/BytecodeLayer/Exec.lean
@@ -5,6 +5,7 @@ import BytecodeLayer.Exec.CallRealises
 import BytecodeLayer.Exec.CleanHaltExtract
 import BytecodeLayer.Exec.CallPreservesSelf
 import BytecodeLayer.Exec.Gas
+import BytecodeLayer.Exec.Alignment
 
 namespace BytecodeLayer.Exec
 
